\documentclass[11pt]{article}
\newtheorem{theorem}{Theorem}
\def\turn{\vdash}
\title{\textbf{\LaTeX\ for Logic}}
\author{AMK}
\begin{document}
\maketitle
\begin{theorem}[belong] $ a, \neg a, \neg b \turn b $.\\
\end{theorem}
\begin{theorem}[not_cancellation] $ a, \neg a, \neg b \turn b $.\\
\end{theorem}
\begin{theorem}[not_introduction] $ a, \neg a, \neg b \turn b $.\\
\end{theorem}
\begin{theorem}[contain_cancellation] $ a, \neg a, \neg b \turn b $.\\
\end{theorem}
\begin{theorem}[contain_introduction] $ a, \neg a, \neg b \turn b $.\\
\end{theorem}
\begin{theorem}[vee_cancellation] $ a, \neg a, \neg b \turn b $.\\
\end{theorem}
\begin{theorem}[vee_introduction_right] $ a, \neg a, \neg b \turn b $.\\
\end{theorem}
\begin{theorem}[vee_introduction_left] $ a, \neg a, \neg b \turn b $.\\
\end{theorem}
\begin{theorem}[wedge_cancellation_left] $ a, \neg a, \neg b \turn b $.\\
\end{theorem}
\begin{theorem}[wedge_cancellation_right] $ a, \neg a, \neg b \turn b $.\\
\end{theorem}
\begin{theorem}[wedge_introduction] $ a, \neg a, \neg b \turn b $.\\
\end{theorem}
\begin{theorem}[contain_cancellation_left] $ a, \neg a, \neg b \turn b $.\\
\end{theorem}
\begin{theorem}[contain_cancellation_right] $ a, \neg a, \neg b \turn b $.\\
\end{theorem}
\begin{theorem}[contain_introduction] $ a, \neg a, \neg b \turn b $.\\
\end{theorem}
\begin{theorem}[wrong_infer] $ a, \neg a, \neg b \turn b $.\\
$(e4)a, \neg a, \neg b \turn b \hfill belong  $\\
$(e5)a, \neg a, \neg b \turn b \hfill not_cancellation (x)(x) $\\
$((null))a, \neg a, \neg b \turn b \hfill contain_introduction  $\\
\end{theorem}
\begin{theorem}[fist proof] $ a, \neg a, \neg b \turn b $.\\
$(1)a, \neg a, \neg b \turn b \hfill belong $\\
$(2)a, \neg a, \neg b \turn \neg a \hfill belong $\\
$(3)a, \neg a, \neg b \turn b \hfill not \_ cancellation (1)(2) $\\
\end{theorem}
\begin{theorem}[second proof] $ a, \neg a, \neg b \turn b $.\\
$(1)a, \neg a, \neg b \turn b \hfill belong $\\
$(2)a, \neg a, \neg b \turn \neg a \hfill belong $\\
$(3)a, \neg a, \neg b \turn b \hfill not \_ cancellation (1)(2) $\\
\end{theorem}
\end{document}
